

Problem 1

a) Claim: let $\hat{n} = \frac{1}{\delta}((1+\delta)^{x_n} - 1)$ then $\mathbb{E}[\hat{n}] = n$

Proof by induction:

Base case ($n=0$)

$$\mathbb{E}[\hat{n}] = \mathbb{E}[(1+\delta)^{x_n} - 1] = (1+\delta)^0 - 1 = 0 = n$$

Inductive case ($n=n+1$)

Assume $\mathbb{E}[\hat{n}] = n$

$$\begin{aligned} \mathbb{E}\left[\frac{1}{\delta}((1+\delta)^{x_{n+1}} - 1)\right] &= \mathbb{E}_{x_0 \dots x_n} \left[\mathbb{E}_{x_{n+1}} \left[\frac{1}{\delta}((1+\delta)^{x_{n+1}} - 1) \right] \right] \\ &= \mathbb{E}_{x_0 \dots x_n} \left[\frac{1}{(1+\delta)^{x_n}} \left(\frac{1}{\delta}((1+\delta)^{x_{n+1}} - 1) \right) + \left(1 - \frac{1}{(1+\delta)^{x_n}} \right) \left(\frac{1}{\delta}((1+\delta)^{x_n} - 1) \right) \right] \\ &= \mathbb{E}_{x_0 \dots x_n} \left[\frac{1}{\delta}((1+\delta) - \frac{1}{(1+\delta)^{x_n}}) + \frac{1}{\delta}((1+\delta)^{x_n} - 1 - 1 + \frac{1}{(1+\delta)^{x_n}}) \right] \\ &= \mathbb{E}_{x_0 \dots x_n} \left[\frac{1}{\delta}((1+\delta) + (1+\delta)^{x_n} - 2) \right] \\ &= \mathbb{E}_{x_0 \dots x_n} \left[\frac{1}{\delta}(\delta + (1+\delta)^{x_n} - 1) \right] \\ &= \mathbb{E}_{x_0 \dots x_n} \left[1 + \frac{1}{\delta}((1+\delta)^{x_n} - 1) \right] \\ &= 1 + n \quad \square \end{aligned}$$

Problem Set 1

Problem 1

b) Claim 1: $V[\hat{n}] \leq \frac{\delta}{2} n^2$

Proof:

$$V[\hat{n}] = E[\hat{n}^2] - E[\hat{n}]^2$$

$$= E_{x_0, \dots, x_n} \left[\frac{1}{\delta^2} ((1+\delta)^{x_n} - 1)^2 \right] - n^2$$

$$= \frac{1}{\delta^2} E_{x_0, \dots, x_n} \left[(1+\delta)^{2x_n} + 1 - 2(1+\delta)^{x_n} \right] - n^2$$

$$E_{x_0, \dots, x_n} [(1+\delta)^{x_n}] = E_{x_0, \dots, x_{n-1}} \left[\frac{1}{(1+\delta)^{x_{n-1}}} (1+\delta)^{x_{n-1}+1} + \left(1 - \frac{1}{(1+\delta)^{x_{n-1}}}\right) (1+\delta)^{x_{n-1}} \right]$$

$$= E_{x_0, \dots, x_{n-1}} \left[(1+\delta) - 1 + (1+\delta)^{x_{n-1}} \right] \rightarrow \text{recursion where } E_{x_0} [(1+\delta)^{x_0}] = 1$$

$$= \delta n + 1$$

$$E_{x_0, \dots, x_n} [(1+\delta)^{2x_n}] = E_{x_0, \dots, x_{n-1}} \left[\frac{1}{(1+\delta)^{2x_{n-1}}} (1+\delta)^{2(x_{n-1}+1)} + \left(1 - \frac{1}{(1+\delta)^{2x_{n-1}}}\right) (1+\delta)^{2x_{n-1}} \right]$$

$$= E_{x_0, \dots, x_{n-1}} \left[(1+\delta)^2 (1+\delta)^{2x_{n-1}} + (1+\delta)^{2x_{n-1}} - (1+\delta)^{2x_{n-1}} \right]$$

$$= E_{x_0, \dots, x_{n-1}} \left[(\delta^2 + 2\delta) (1+\delta)^{2x_{n-1}} + (1+\delta)^{2x_{n-1}} \right]$$

$$= (\delta^2 + 2\delta) (\delta n + 1) + E[(1+\delta)^{2x_{n-1}}] \rightarrow \text{recursion where } E[(1+\delta)^{2x_0}] = 1$$

$$= (\delta^2 + 2\delta) \left[\sum_{i=1}^{n-1} [\delta(n-i) + 1] + 1 \right]$$

from prev. calculation from final term

$$= (\delta^2 + 2\delta) \left(\frac{\delta n(n-1)}{2} + (n-1) + 1 \right)$$

$$= \frac{\delta^2(\delta+2)n(n-1)}{2} + (\delta^2+2\delta)n$$

$$V[\hat{n}] = \frac{1}{\delta^2} \left(\frac{\delta^2(\delta+2)(n-1)n}{2} + (\delta^2+2\delta)n + 1 - 2(\delta n + 1) \right) - n^2$$

$$= \frac{n}{2} (\delta n - \delta + 2n - 2) + n + \frac{2n}{\delta} + \frac{1}{\delta^2} - \frac{2n}{\delta} - \frac{2}{\delta^2} - n^2$$

$$= \frac{\delta n^2}{2} - \frac{\delta n}{2} + n^2 - n + n + \frac{1}{\delta^2} - n^2$$

$$= \frac{\delta}{2} n^2 - \frac{\delta}{2} n - \frac{1}{\delta^2}$$

$$\leq \frac{\delta}{2} n^2$$

□

Problem Set 1

Problem 1

b) Claim 2: $P[|\hat{n} - n| \leq \epsilon n] \geq .9$ as long as $\delta \leq \frac{\epsilon^2}{5}$

Proof:

From Chebyshev's Inequality,

$$P[|\hat{n} - n| \geq \lambda] \leq \frac{V[\hat{n}]}{\lambda^2}$$

$$P[|\hat{n} - n| \leq \lambda] \geq 1 - \frac{V[\hat{n}]}{\lambda^2}$$

$$\text{let } \lambda^2 = 10 V[\hat{n}]$$

$$P[|\hat{n} - n| \leq \sqrt{10 V[\hat{n}]}] \geq .9$$

$$\sqrt{10 V[\hat{n}]} \leq \sqrt{10 \frac{\delta}{2} n^2} = \sqrt{5\delta} n$$

$$\epsilon = \sqrt{5\delta}$$

$$\delta = \frac{\epsilon^2}{5} = \boxed{.2 \epsilon^2}$$

c) Claim: space required is $O(\lg \lg n + \lg \frac{1}{\epsilon})$

Proof: space $\leq O(\lg x_n)$

$$\frac{(1+\delta)^{x_n} - 1}{\delta} \leq (1+\epsilon)n$$

$$x_n \leq \lg_{(1+\delta)} ((1+\epsilon)n\delta + 1)$$

$$\text{so space} \leq O(\lg \lg_{(1+\delta)} ((1+\epsilon)n\delta + 1))$$

$$= O(\lg \left(\frac{\lg(n\delta + \epsilon n\delta + 1)}{\lg(1+\delta)} \right))$$

$$= O(\lg \lg n - \lg \lg(1+\epsilon^2))$$

$$\rightarrow = O(\lg \lg n - \lg \epsilon^2) \quad \text{from Taylor Series}$$

$$= O(\lg \lg n + \lg \frac{1}{\epsilon})$$

□

We know $\epsilon \in (0,1)$
 ϵ^2 is small and close to 0. The Taylor Approximation is below.

$$\lg(1+x) \approx \lg(1) + \frac{1}{1+0}(x) - \frac{1}{2} \frac{1}{(1+0)^2}(x^2) \dots$$

$$= O(x - \frac{x^2}{2} + \dots)$$

$$= O(x)$$

Problem Set 1

Problem 2

a) Claim: $\forall x \neq y, x, y \in U, P[h(x) = h(y)] = \frac{1}{n}$

Proof: Let $x, y \in U$ s.t. $x \neq y$

Consider 4 cases

- | | | | |
|----------------|-------------------|----------------|-------------------|
| 1. $x_H = y_H$ | 2. $x_H \neq y_H$ | 3. $x_H = y_H$ | 4. $x_H \neq y_H$ |
| $x_L = y_L$ | $x_L = y_L$ | $x_L \neq y_L$ | $x_L \neq y_L$ |

Case 1:

Impossible since $x \neq y$ by definition

Case 2. $P[h(x) = h(y)] = P[H[x_H] \oplus L[x_L] = H[y_H] \oplus L[y_L]]$

$$= P[H[x_H] = H[y_H]] \quad \text{since we know } L[x_L] = L[y_L]$$

there are $n^{u/2}$ possible $H[\cdot]$ arrays

$n^{u/2-1}$ possible where $H[x_H] = H[y_H]$

$$= \frac{n^{u-1}}{n^u} = \frac{1}{n}$$

Case 3.

Same as case 2 by symmetry

Case 4. $P[H[x_H] \oplus L[x_L] = H[y_H] \oplus L[y_L]]$

$$= P[H[x_H] \oplus H[y_H] = L[x_L] \oplus L[y_L]] \quad \text{bc. of how xor works}$$

Consider the $P[H[x_H] \oplus H[y_H] = a]$ where $a \in \{0, \dots, n-1\}$

This is essentially the same as case 2, since for any $H[x_H]$ and a there is only one $H[y_H]$ that works. The same reasoning applies to $L[\cdot]$ by symmetry.

$$P[H[x_H] \oplus H[y_H] = L[x_L] \oplus L[y_L]]$$

$$= \sum_{a=0}^{n-1} P[H[x_H] \oplus H[y_H] = a] \cdot P[L[x_L] \oplus L[y_L] = a]$$

$$= \sum_{a=0}^{n-1} \frac{1}{n} \cdot \frac{1}{n} = \frac{n}{n^2} = \frac{1}{n}$$

In every case, the claim holds true \square

Problem Set 1

Problem 2

b) Claim: $\forall x \neq y, x, y \in V \quad P[h(x) = h(y)] = \frac{1}{n}$

Proof: let $b \in \{2, \dots, u\}$ be the number of $H[\cdot]$ arrays
this is also the number of pieces on input to $h(\cdot)$
will be split into.

Base case: $b=2$

This is the hash function from part a which we have proved is universal.

Inductive case: $b=b+1$

Assume a hash function with b arrays is universal

$$P[h(x) = h(y)] = P[H_1[x_1] \oplus \dots \oplus H_b[x_b] \oplus H_{b+1}[x_{b+1}] = H_1[y_1] \oplus \dots \oplus H_b[y_b] \oplus H_{b+1}[y_{b+1}]]$$

let $x_h = x[0:b]$ bits, $y_h = y[0:b]$ bits

Case 1. $x_h = y_h, x_{b+1} = y_{b+1}$: Impossible by definition

Case 2. $x_h = y_h, x_{b+1} \neq y_{b+1}$

$$P[h(x) = h(y)] = P[H_{b+1}[x_{b+1}] = H_{b+1}[y_{b+1}]]$$

number of possible $H_{b+1} = n^{2^{\frac{u}{b}}}$

number of possible where $H_{b+1}[x_{b+1}] = H_{b+1}[y_{b+1}] = n^{2^{\frac{u}{b}-1}}$

$$P[h(x) = h(y)] = \frac{n^{2^{\frac{u}{b}-1}}}{n^{2^{\frac{u}{b}}}} = \frac{1}{n}$$

Case 3. $x_h \neq y_h, x_{b+1} = y_{b+1}$

$$P[h(x) = h(y)] = \frac{1}{n} \text{ by induction hypothesis}$$

Problem Set 1

Problem 2

b) Case 4: $X_n \neq Y_n, X_{b+1} \neq Y_{b+1}$

$$\begin{aligned} P[h(X) = h(Y)] &= P[H_1[X_1] \oplus \dots \oplus H_b[X_b] \oplus H_1[Y_1] \oplus \dots \oplus H_b[Y_b] \\ &= H_{b+1}[X_{b+1}] \oplus H_{b+1}[Y_{b+1}]] \end{aligned}$$

$$= \sum_{a=0}^{n-1} P[H_1[X_1] \oplus \dots \oplus H_b[Y_b] = a] \cdot P[H_{b+1}[X_{b+1}] \oplus H_{b+1}[Y_{b+1}]]$$

$$= \sum_{a=0}^{n-1} \frac{1}{n} \cdot \frac{1}{n} = \frac{n}{n^2} = \frac{1}{n}$$

This is because the first term is a restatement of our induction hypothesis. Checking equivalence is just the special case where $a=0$. The second term is $\frac{1}{n}$ following the same logic in case 2.

The claim holds in every case, so by induction it will be true when $b=n$ \square

The space to specify the hash function is

$$O(u \cdot 2 \cdot \lg n) = O(u \lg n)$$

from u arrays with two numbers taking $\lg n$ bits each.

Problem Set 1

Problem 3

a) Let X_i be the number of elements mapped to bucket i

Claim: $P[X_i \geq w] \geq \frac{1}{\sqrt{n}}$ where $w = c \frac{\lg n}{\lg \lg n}$, $c > 0$

$$\begin{aligned} \text{Proof: } P[X_i \geq w] &= \sum_{i=w}^n P[X_i = i] = \sum_{i=w}^n \binom{n}{i} \left(\frac{1}{n}\right)^i \left(\frac{n-1}{n}\right)^{n-i} \\ &\geq \binom{n}{w} \left(\frac{1}{n}\right)^w \left(\frac{n-1}{n}\right)^{n-w} \quad \text{just the largest term} \\ &\geq \left(\frac{n}{w}\right)^w \left(\frac{1}{n}\right)^w \left(\frac{n-1}{n}\right)^{n-w} \quad \text{from Stirling's inequality} \\ &\geq \left(\frac{1}{w}\right)^w \left(\frac{n-1}{n}\right)^{n-w} \end{aligned}$$

$$\left(\frac{n-1}{n}\right)^{n-w} \geq \left(1 - \frac{1}{n}\right)^n \rightarrow e^{-1} \text{ as } n \rightarrow \infty \text{ by definition of } e$$

when $n \geq 2$ $\left(\frac{n-1}{n}\right)^n \geq \frac{1}{4}$ and is upper-bounded by $\frac{1}{e}$

$$\begin{aligned} \text{Therefore } P[X_i \geq w] &\geq \frac{1}{4} \left(\frac{1}{w}\right)^w = \frac{1}{4} w^{-w} \\ &\geq 2^{\lg(\frac{1}{4} w^{-w})} = 2^{-w \lg(\frac{4}{w})} \end{aligned}$$

Let c be a small constant such as $\frac{1}{1000}$

$$\geq 2^{-\frac{1}{1000} \frac{\lg n}{\lg \lg n} (\lg \lg n - \lg 4000 \lg \lg n)}$$

$$\geq 2^{-\frac{1}{1000} \lg n} \quad \text{by dropping the positive exponent term}$$

$$\geq n^{-\frac{1}{1000}} \geq n^{-\frac{1}{2}}$$

□

Problem Set 1

Problem 3

b) Claim: Let X be the number of heavy buckets
 $\mathbb{E}[X] = \Omega(\sqrt{n})$

$$\begin{aligned}\text{Proof: } \mathbb{E}[X] &= \mathbb{E}\left[\sum_{i=1}^n \mathbb{1}[X_i \geq \sqrt{n}]\right] \\ &= \sum_{i=1}^n \mathbb{P}[X_i \geq \sqrt{n}] \\ &\geq \sum_{i=1}^n \frac{1}{\sqrt{n}} \\ &\geq \frac{n}{\sqrt{n}} = \sqrt{n}\end{aligned}$$

Therefore, X is lower bounded by \sqrt{n} and
 $\mathbb{E}[X] = \Omega(\sqrt{n})$

□